towards typing and extraction

examples/low-level/crypto/Crypto.AEAD.Chacha20Poly1305.fst
@@ -11,7 +11,6 @@ open Crypto.Symmetric.Chacha20
 module Spec = Crypto.Symmetric.Poly1305.Spec
 module MAC = Crypto.Symmetric.Poly1305.MAC
 
-//#set-options "--lax"
 
 (* If the length is not a multipile of 16, pad to 16 *)
 val pad_16: b:bytes -> len:UInt32.t -> STL unit
@@ -37,9 +36,8 @@ let upd_uint32 b x : STL unit
   upd b 2ul v2;
   upd b 3ul v3
 
-
 (* Serializes the lengths into the appropriate format *)
-val length_bytes: b:bytes -> len:UInt32.t -> aad_len:UInt32.t -> STL unit
+private val length_bytes: b:bytes -> len:UInt32.t -> aad_len:UInt32.t -> STL unit
   (requires (fun h -> live h b /\ length b >= 16))
   (ensures  (fun h0 _ h1 -> live h1 b /\ modifies_1 b h0 h1))
 let length_bytes b len aad_len =
@@ -47,51 +45,41 @@ let length_bytes b len aad_len =
   upd_uint32 (offset b  4ul) 0ul;
   upd_uint32 (offset b  8ul) aad_len;
   upd_uint32 (offset b 12ul) 0ul
-  
 
-val mac_inv:
+
+private val add_bytes:
   #i: MAC.id ->
   st: MAC.state i ->
-  l0: MAC.ilog -> 
-  a : MAC.accB i -> 
-  h:HyperStack.mem -> Type0
-
-val isel: l:MAC.ilog {MAC.ideal} -> Tot (Seq.seq Spec.elem)
-// let isel l = 
-// match MAC.ideal with | true -> let log: Seq.seq Spec.elem = l in l
-
-let mac_inv #i st l0 a h = 
-  let r = MAC.State.r st in (
-  live h a /\ 
-  live h r /\
-  MAC.norm h a /\ 
-  MAC.norm h r /\
-  (MAC.ideal ==> (
-    MAC.sel_elem h a = Spec.poly (isel l0) (MAC.sel_elem h r))))
-
-
-val add_bytes:
-  #i: MAC.id ->
-  st: MAC.state i ->
-  l0: MAC.ilog -> 
+  l0: MAC.itext -> 
   a : MAC.accB i ->
-  txt:bytes -> STL MAC.ilog
+  l : UInt32.t ->
+  txt:bytes { length txt = v l } -> STL MAC.itext
   (requires (fun h -> 
-    live h txt /\ mac_inv st l0 a h))
+    live h txt /\ MAC.acc_inv st l0 a h))
   (ensures (fun h0 l1 h1 -> 
     modifies_1 a h0 h1 /\ 
     live h1 txt /\ 
-    l1 = MAC.encode_pad l0 (MAC.sel_bytes h0 txt) /\
-    mac_inv st l1 a h1))
+//?    (MAC.ideal ==> l1 = MAC.encode_pad l0 (MAC.sel_bytes h0 txt)) /\
+    MAC.acc_inv st l1 a h1))
 
-let rec loop #i st l0 a txt ctr =
-  if ctr = 0 then l0 else 
-  begin
-    let w = sub txt 0ul 16ul in
-    let l1 = add st l0 a w in 
-    let txt1 = offset txt 16ul in
-    loop st l1 a txt1 (ctr - 1)
-  end
+let rec add_bytes #i st log a l txt =
+  assume false; //TODO
+  if l = 0ul then log 
+  else if l <^ 16ul then 
+    begin
+      let w = create 0uy 16ul in
+      blit txt 0ul w 0ul l;
+      pad_16 w (16ul -^ l);
+      MAC.add st log a w
+    end
+  else 
+    begin
+      let w = Buffer.sub txt 0ul 16ul in 
+      let l = MAC.add st log a w in
+      let txt = offset txt 16ul in 
+      add_bytes st log a l txt 
+    end
+
 
 (* AEAD-encrypt for Chacha20-Poly1305. Takes:
    - the additional data (aad)
@@ -115,11 +103,12 @@ val chacha20_aead_encrypt: ciphertext:bytes -> tag:bytes -> aad:bytes -> key:byt
   ))
   (ensures (fun h0 _ h1 -> live h1 ciphertext /\ live h1 tag /\ modifies_2 ciphertext tag h0 h1 ))
 let chacha20_aead_encrypt ciphertext tag aad key iv constant plaintext len aad_len =
+  assume false; //TODO
   push_frame();
 
   (* Temporary buffers (to be improved) *)
   let state = create 0ul 32ul in (* Chacha inner state *)
-  chacha20_init state key counter iv constant;
+  chacha20_init state key 0ul iv constant;
 
   (*  Create OTK, using round '0' of Chacha20 *)
   let counter = 0ul in
@@ -130,46 +119,30 @@ let chacha20_aead_encrypt ciphertext tag aad key iv constant plaintext len aad_l
   let counter = 1ul in
   chacha20_encrypt ciphertext key counter iv constant plaintext len;
 
-  (*  MACing of the additional data, the ciphertext and the padding *)
-  (* Compute the padding lengths *)
-  let max = UInt32.div len 16ul in
-  let rem = UInt32.rem len 16ul in
-  let max_aad = UInt32.div aad_len 16ul in
-  let rem_aad = UInt32.rem aad_len 16ul in
-  (* Create padded blocks *)
-  let padded_aad = create 0uy 16ul in
-  let padded_ciphertext = create 0uy 16ul in
-  let len_bytes = create 0uy 16ul in
-  blit ciphertext (UInt32.mul max 16ul) padded_ciphertext 0ul rem;
-  pad_16 padded_ciphertext rem; // not needed, unless buffer reuse
-  blit aad (UInt32.mul max_aad 16ul) padded_aad 0ul rem_aad;
-  pad_16 padded_aad rem_aad;    // not needed, unless buffer reuse
-
   (* Initialize MAC algorithm with one time key *)
   (* encapsulate (r,s) and a; we should probably clear otk *)
-  let ak = MAC.coerce root otk in 
+  let ak = MAC.coerce MAC.someId HyperHeap.root otk in 
   let acc = MAC.start ak in
-
-  (* the log is a sequence of abstract elements that encode the message *)
 
   (* Update MAC with
      - padded additional data
      - padded ciphertext
      - formatted length *)
-  let log = 
-    let log = MAC.loop MAC.log_0 aad acc r max_aad in
-    (* This is not length-constant time, the lengths are assumed to 
-       be public data *)  
-    if not(UInt32.eq rem_aad 0ul) then poly1305_update log padded_aad acc r
-    else log in
-  let aad_ciphertext_log = 
-    let log = poly1305_loop aad_log ciphertext acc r max in
-    if not(UInt32.eq rem 0ul) then poly1305_update log padded_ciphertext acc r
-    else log in
-  length_bytes len_bytes len aad_len;
-  let full_log = poly1305_update aad_ciphertext_log len_bytes acc r in
+  (* the log is a sequence of abstract elements that encode the message *)
+  (* This is not length-constant time, the lengths are assumed to be public data *)  
+
+  let final_word = create 0uy 16ul in 
+  length_bytes final_word len aad_len;
+
+  let l = MAC.text_0 in 
+  let l = add_bytes ak l acc aad_len aad in
+  let l = add_bytes ak l acc len ciphertext in 
+  let l = MAC.add ak l acc final_word in
+  
   (* Finish MAC *)
-  poly1305_finish tag acc (Buffer.sub otk 16ul 16ul);
+  MAC.mac ak l acc tag;
+  
   pop_frame()
 
   
+//TODO: decryption!
